LogRel/LemmasInversion.v
@@ -273,24 +273,3 @@ Section ValrelInversion.
       exact (invert_valrel_pEmulDV_inArr vr).
   Qed.
 End ValrelInversion.
-
-(* Section DestructUVal. *)
-(*   Lemma termrel_caseUValUnit {d w n p vs vu}:  *)
-(*     dir_world_prec d w n p → *)
-(*     valrel d w (pEmulDV (S n) p) vs vu → *)
-(*     termrel d w ptunit (caseUValUnit n vs) (seq vu unit). *)
-(*   Proof. *)
-(*     unfold caseUValUnit. *)
-(*     intros vr. *)
-(*     destruct (valrel_implies_Value vr). *)
-(*     apply invert_valrel_pEmulDV in vr. *)
-(*     destruct vr as [[? ?] | other_cases]; subst. *)
-(*     - admit. *)
-(*     - destruct other_cases as (? & [ [? vr] | [ [? vr] | [ [? vr] | [[? vr] | [? vr]]]]]); *)
-(*       eapply termrel_antired_star; *)
-(*       eauto using caseUVal_eval_unk, caseUVal_eval_unit, caseUVal_eval_bool, caseUVal_eval_prod, caseUVal_eval_sum, caseUVal_eval_arr,  *)
-(*       valrel_in_termrel, valrel_inUnit'. *)
-      
-(*   Qed. *)
-
-(* End DestructUVal. *)
